***NO_CI*** Shallow verifies against the new interface; added allocation

examples/seplogic/Shallow.fst
@@ -24,16 +24,14 @@ let return (#a:Type) (x:a)
   = fun post h0 -> FStar.Squash.return_squash (x, h0)
 
 (* frame wp by partitioning a heap whose memory is m into h0 and h1, and then prove post on the resulting heap and h1 *)
-let frame_wp0 (#a:Type) (wp:st_wp a) (post:memory -> (a * memory) -> Type0) (m:memory) (h0 h1:heap) =
-  let m0 = heap_memory h0 in
-  let m1 = heap_memory h1 in 
+let frame_wp0 (#a:Type) (wp:st_wp a) (post:memory -> (a * memory) -> Type0) (m m0 m1:memory) =
   disjoint_memories m0 m1 /\ m == (m0 <*> m1) /\ wp (post m1) m0
 
-let frame_wp1 (#a:Type) (wp:st_wp a) (post:memory -> (a * memory) -> Type0) (m:memory) (h0:heap) =
-  exists (h1:heap). frame_wp0 wp post m h0 h1
+let frame_wp1 (#a:Type) (wp:st_wp a) (post:memory -> (a * memory) -> Type0) (m m0:memory) =
+  exists (m1:memory). frame_wp0 wp post m m0 m1
 
 let frame_wp (#a:Type) (wp:st_wp a) (post:memory -> (a * memory) -> Type0) (m:memory) =
-  exists (h0:heap). frame_wp1 wp post m h0
+  exists (m0:memory). frame_wp1 wp post m m0
 
 (* the idea is to call frame_wp with (frame_post p)? yes, see frame below *)
 let frame_post (#a:Type) (p:post a) (m0:memory) ((x, m1):(a * memory)) = disjoint_memories m0 m1 /\ p (x, m0 <*> m1)
@@ -52,15 +50,18 @@ let bind_exists
 val frame: #a:Type -> #wp:st_wp a -> f:st a wp
          -> st a (fun post -> frame_wp wp (frame_post post))
 //Expanded out:
-//         st a (fun post m -> exists m0 m1. disjoint m0 m1 /\ m == m0 <*> m1 /\ wp (fun m0' -> disjoint m0' m1 /\ post (x, (join_tot m0' m1))) m0
+//         st a (fun post m -> exists m0 m1. disjoint m0 m1 /\ m == m0 <*> m1 /\ wp (fun m0' -> disjoint m0' m1 /\ post (x, (join_tot h0' h1))) m0
 let frame #a #wp f = 
   fun post h ->
     assert (frame_wp wp (frame_post post) (heap_memory h));
     let s = FStar.Squash.join_squash (FStar.Squash.get_proof (frame_wp wp (frame_post post) (heap_memory h))) in
-    bind_exists #(result a post) #heap #(frame_wp1 wp (frame_post post) (heap_memory h)) s (fun h0 s' -> 
-      assert (frame_wp1 wp (frame_post post) (heap_memory h) h0);
-      bind_exists #(result a post) #heap #(frame_wp0 wp (frame_post post) (heap_memory h) h0) s' (fun h1 _ -> 
-        assert (frame_wp0 wp (frame_post post) (heap_memory h) h0 h1);
+    bind_exists #(result a post) #memory #(frame_wp1 wp (frame_post post) (heap_memory h)) s (fun m0 s' -> 
+      assert (frame_wp1 wp (frame_post post) (heap_memory h) m0);
+      bind_exists #(result a post) #memory #(frame_wp0 wp (frame_post post) (heap_memory h) m0) s' (fun m1 _ -> 
+        assert (frame_wp0 wp (frame_post post) (heap_memory h) m0 m1);
+        assert (disjoint_memories m0 m1);
+        assert (heap_memory h == (m0 <*> m1));
+        let (h0,h1) = split_heap m0 m1 h in
         let sqres : squash (result a (frame_post post (heap_memory h1))) = f (frame_post post (heap_memory h1)) h0 in 
         S.bind_squash #(result a (frame_post post (heap_memory h1)))
                       #(result a post)
@@ -69,7 +70,7 @@ let frame #a #wp f =
                          let (x, h0') = x_h0' in
                          let res = (x, join_tot h1 h0') in 
                          FStar.Squash.return_squash res)))
-
+      
 val bind (#a:Type) (#wp1:st_wp a)
          (#b:Type) (#wp2:a -> st_wp b)
          (f:st a wp1)
@@ -85,13 +86,10 @@ let bind #a #wp1 #b #wp2 f g =
       frame (g x) post m1)
 
 let alloc (#a:Type0) (x:a)
-  : st (ref a) (fun post m0 -> m0 == emp /\ (exists (r:ref a) . post (r, (r |> x))))
+  : st (ref a) (fun post m0 -> m0 == emp /\ (forall r m1 . m1 == (r |> x) ==> post (r, m1)))
   = fun post h0 ->
-      assert (heap_memory h0 == emp);
       let (r,h1) = alloc h0 x in
-      assert (heap_memory h1 == (r |> x));
-      admit ()
-      //FStar.Squash.return_squash ()
+      FStar.Squash.return_squash (r,h1)
 
 let read (#a:Type0) (r:ref a)
   : st a (fun post m0 -> (exists (x:a). m0 == (r |> x) /\ post (x, m0)))
@@ -100,7 +98,7 @@ let read (#a:Type0) (r:ref a)
       FStar.Squash.return_squash (sel_tot h0 r, h0)
 
 let write (#a:Type0) (r:ref a) (v:a)
-  : st unit (fun post m0 -> (exists (x:a). m0 == (r |> x) /\ (forall m1. m1 == (r |> v) ==> post ((), m1))))
+  : st unit (fun post m0 -> (exists (x:a). m0 == (r |> x) /\ post ((), (r |> v))))
     = fun post h0 -> 
         assert (mcontains (heap_memory h0) r);
         FStar.Squash.return_squash ((), upd_tot h0 r v)
