examples/seplogic/SepLogic.HeapMemory.fsti
@@ -9,6 +9,8 @@ let tset = TSet.set
 val heap : Type u#1
 val memory : Type u#1
 
+val emp : memory
+
 val ref (a:Type0) : Type0
 val addr_of : #a:Type0 -> ref a -> GTot nat
 
@@ -21,20 +23,56 @@ let mpred = memory -> Type0
 val disjoint_heaps : heap -> heap -> Type0
 val disjoint_memories : memory -> memory -> Type0
 
+val disjoint_heaps_comm (h0 h1:heap)
+  : Lemma (disjoint_heaps h0 h1 <==> disjoint_heaps h1 h0)
+
+val disjoint_memories_emp (m:memory)
+  : Lemma (disjoint_memories m emp)
+          [SMTPat (disjoint_memories m emp)]
+
+val disjoint_memories_comm (m0 m1:memory)
+  : Lemma (disjoint_memories m0 m1 <==> disjoint_memories m1 m0)
+
 val disjoint_heaps_memories (h0 h1:heap)
   : Lemma (disjoint_heaps h0 h1 <==> disjoint_memories (heap_memory h0) (heap_memory h1))
           [SMTPat (disjoint_memories (heap_memory h0) (heap_memory h1))]
 
-val emp : memory
+val join_tot: h0:heap -> h1:heap{disjoint_heaps h0 h1} -> Tot heap
+
+val join_tot_comm (h0 h1:heap)
+  : Lemma (requires (disjoint_heaps h0 h1 /\ disjoint_heaps h1 h0))
+          (ensures  (join_tot h0 h1 == join_tot h1 h0))
+
 val ( |> ) : #a:Type0 -> r:ref a -> x:a -> memory
 val ( <*> ) : m0:memory -> m1:memory{disjoint_memories m0 m1} -> memory
-
-val join_tot: h0:heap -> h1:heap{disjoint_heaps h0 h1} -> Tot heap
 
 val sep_join_tot (h0 h1:heap)
   : Lemma (requires (disjoint_heaps h0 h1))
           (ensures  (heap_memory (join_tot h0 h1) == ((heap_memory h0) <*> (heap_memory h1))))
           [SMTPat (heap_memory (join_tot h0 h1))]
+
+val split_heap : (m0:memory) 
+              -> (m1:memory{disjoint_memories m0 m1})
+              -> (h:heap{heap_memory h == (m0 <*> m1)}) 
+              -> heap * heap
+
+val split_heap_disjoint (m0 m1:memory) (h:heap)
+  : Lemma (requires (disjoint_memories m0 m1 /\ heap_memory h == (m0 <*> m1)))
+          (ensures  (let (h0,h1) = split_heap m0 m1 h in
+                     disjoint_heaps h0 h1))
+          [SMTPat (split_heap m0 m1 h)]
+
+val split_heap_join_tot (m0 m1:memory) (h:heap)
+  : Lemma (requires (disjoint_memories m0 m1 /\ heap_memory h == (m0 <*> m1)))
+          (ensures  (let (h0,h1) = split_heap m0 m1 h in
+                     h == join_tot h0 h1))
+          [SMTPat (split_heap m0 m1 h)]
+
+val split_heap_memories (m0 m1:memory) (h:heap)
+  : Lemma (requires (disjoint_memories m0 m1 /\ heap_memory h == (m0 <*> m1)))
+          (ensures  (let (h0,h1) = split_heap m0 m1 h in
+                     heap_memory h0 == m0 /\ heap_memory h1 == m1))
+          [SMTPat (split_heap m0 m1 h)]
 
 val hcontains : #a:Type0 -> heap -> ref a -> Type0
 val mcontains : #a:Type0 -> memory -> ref a -> Type0
@@ -98,152 +136,3 @@ val alloc_emp_points_to (#a:Type0) (h0:heap) (x:a)
 
 
 
-
-(*
-//let hpred = heap -> Type0
-
-val emp :heap
-
-// val join_tot: h1:heap -> h2:heap -> Tot heap
-
-// val join_tot_comm (h0:heap) (h1:heap)
-//   : Lemma (join_tot h0 h1 == join_tot h1 h0)
-
-val disjoint : #a:Type0 -> #b:Type0 -> ref a -> ref b -> Type0
-
-val disjoint_comm (#a:Type0) (#b:Type0) (r0:ref a) (r1:ref b)
-  : Lemma (requires (disjoint r0 r1))
-          (ensures  (disjoint r1 r0))
-
-val disjoint_heaps : heap -> heap -> Type0
-
-// val disjoint_heaps_emp (h0 h1:heap)
-//   : Lemma (requires (emp h1)) 
-//           (ensures  (disjoint_heaps h0 h1))
-//           [SMTPat (disjoint_heaps h0 h1); 
-//            SMTPat (emp h1)]
-
-val disjoint_heaps_comm (h0 h1:heap)
-  : Lemma (requires (disjoint_heaps h0 h1))
-          (ensures  (disjoint_heaps h1 h0))
-
-val ( |> ) :#a:Type0 -> r:ref a -> x:a -> heap
-val ( <*> ) :heap -> heap -> heap
-
-// val ( |> ) : #a:Type0 -> r:ref a -> x:a -> hpred
-// val ( <*> ) : hpred -> hpred -> hpred
-
-// val sep_interp (p q:hpred) (h:heap)
-//   : Lemma ((p <*> q) h <==> (exists h0 h1. disjoint_heaps h0 h1 /\ h == join_tot h0 h1 /\ p h0 /\ q h1))
-
-val sep_emp (h:heap)
-  :Lemma (requires True)
-         (ensures (h <*> emp) == h)
-         [SMTPat (h <*> emp)]
-
-val sep_comm (h1 h2:heap)
-  :Lemma (requires True)
-         (ensures ((h1 <*> h2) == (h2 <*> h1)))
-	 [SMTPat (h1 <*> h2)]
-
-val sep_assoc (h1 h2 h3:heap)
-  :Lemma (requires True)
-         (ensures (h1 <*> (h2 <*> h3)) == (h2 <*> (h1 <*> h3)))
-	 [SMTPatOr [[SMTPat (h1 <*> (h2 <*> h3))]; [SMTPat (h2 <*> (h1 <*> h3))]]]
-         
-*)
-
-// val fresh : #a:Type0 -> ref a -> hpred
-// val contains : #a:Type0 -> heap -> ref a -> Type0
-
-// val points_to_contains (#a:Type0) (r:ref a) (x:a) (h:heap)
-//   : Lemma (requires ((r |> x) h))
-//           (ensures  (h `contains` r))
-//           [SMTPat ((r |> x) h);
-//            SMTPat (h `contains` r)]
-
-// val points_to_ext (#a:Type0) (r:ref a) (x y:a) (h:heap)
-//   : Lemma (requires ((r |> x) h /\ (r |> y) h))
-//           (ensures  (x == y))
-
-// val points_to_disj (#a:Type0) (#b:Type0) (r:ref a) (s:ref b) (x:a) (y:b) (h:heap)
-//     : Lemma (requires ((r |> x <*> s |> y) h))
-//             (ensures  (disjoint r s))
-//             [SMTPat ((r |> x <*> s |> y) h);
-//              SMTPat (disjoint r s)]
-
-// val join_tot_contains (#a:Type0) (r:ref a) (h0 h1:heap) 
-//   : Lemma (requires (h1 `contains` r /\ disjoint_heaps h0 h1))
-//           (ensures  (contains (join_tot h0 h1) r))
-//           [SMTPat (contains (join_tot h0 h1) r)]
-
-// val sel_tot: #a:Type0 -> h:heap -> r:ref a{h `contains` r} -> Tot a
-// val upd_tot: #a:Type0 -> h:heap -> r:ref a{h `contains` r} -> x:a -> Tot heap
-
-// val points_to_sel (#a:Type) (r:ref a) (x:a) (h:heap)
-//   : Lemma (requires (r |> x) h)
-//           (ensures  (sel_tot h r == x))
-//           [SMTPat ((r |> x) h);
-//            SMTPat (sel_tot h r)]
-
-// val points_to_upd (#a:Type) (r:ref a) (x:a) (v:a) (h:heap)
-//   : Lemma  (requires (r |> x) h)
-//            (ensures  ((r |> v) (upd_tot h r v)))
-//            [SMTPat ((r |> x) h);
-//             SMTPat (upd_tot h r v)]
-
-// val restrict: #a:Type0 -> h:heap -> r:ref a{h `contains` r} -> Tot heap
-// val minus: #a:Type0 -> h:heap -> r:ref a{h `contains` r} -> Tot heap
-
-// val minus_not_contains (#a:Type0) (r:ref a) (h:heap)
-//   : Lemma (requires (h `contains` r))
-//           (ensures  (~((h `minus` r) `contains` r)))
-//           [SMTPat ((h `minus` r) `contains` r);
-//            SMTPat (h `contains` r)]
-
-// val restrict_points_to (#a:Type0) (r:ref a) (h:heap)
-//   : Lemma (requires (h `contains` r))
-//           (ensures  (exists x . (r |> x) (restrict h r)))
-//           [SMTPat (restrict h r);
-//            SMTPat (h `contains` r)]
-
-// val disjoint_heaps_restrict_minus (#a:Type0) (r:ref a) (h:heap)
-//   : Lemma (requires (h `contains` r))
-//           (ensures  (disjoint_heaps (restrict h r) (minus h r)))
-//           [SMTPat (disjoint_heaps (restrict h r) (minus h r))]
-
-// val disjoint_heaps_minus_1 (#a:Type0) (r:ref a) (x:a) (h:heap)
-//   : Lemma (requires ((r |> x) h))
-//           (ensures  (disjoint_heaps (minus h r) h))
-//           [SMTPat (disjoint_heaps (minus h r) h);
-//            SMTPat ((r |> x) h)]
-
-// val disjoint_heaps_minus_2 (#a:Type0) (r:ref a) (x0 x1:a) (h0:heap) (h1:heap)
-//   : Lemma (requires ((r |> x0) h0 /\ (r |> x1) h1))
-//           (ensures  (disjoint_heaps (minus h0 r) h1))
-//           [SMTPat (disjoint_heaps (minus h0 r) h1);
-//            SMTPat ((r |> x0) h0);
-//            SMTPat ((r |> x1) h1)]
-
-// val join_tot_restrict_minus (#a:Type0) (r:ref a) (h:heap)
-//   : Lemma (requires (h `contains` r))
-//           (ensures  (join_tot (restrict h r) (minus h r) == h))
-//           [SMTPat (join_tot (restrict h r) (minus h r))]
-
-// val join_tot_minus_restrict (#a:Type0) (r:ref a) (h:heap)
-//   : Lemma (requires (h `contains` r))
-//           (ensures  (join_tot (minus h r) h == restrict h r))
-//           [SMTPat (join_tot (minus h r) h);
-//            SMTPat (restrict h r)]
-
-// val points_to_join_tot_minus (#a:Type0) (r:ref a) (x y:a) (h h':heap)
-//   : Lemma (requires ((r |> x) h /\ (r |> y) h'))
-//           (ensures  ((r |> y) (join_tot (minus h r) h')))
-//           [SMTPat ((r |> x) h);
-//            SMTPat ((r |> y) (join_tot (minus h r) h'))]
-
-// val points_to_join_tot_restrict (#a:Type0) (r:ref a) (x y:a) (h h':heap)
-//   : Lemma (requires ((r |> x) h /\ (r |> y) h'))
-//           (ensures  ((r |> y) (restrict (join_tot (minus h r) h') r)))
-//           [SMTPat ((r |> x) h);
-//            SMTPat ((r |> y) (restrict (join_tot (minus h r) h') r))]
